work on making inductive type definitions (broke build)

coc-rs/src/inductive_type.rs
@@ -1,0 +1,238 @@
+use crate::term::RecursiveTermKind::*;
+use crate::term::{RecursiveTermKind, Term, TermRef};
+use extend::ext;
+use std::collections::HashMap;
+use std::iter;
+
+pub trait ConstructUsingNames {
+    fn forall(argument_name: Option<String>, argument_type: Self, return_type: Self) -> Self;
+    fn lambda(argument_name: Option<String>, argument_type: Self, return_value: Self) -> Self;
+    fn apply(f: Self, argument: Self) -> Self;
+    fn variable_impl(name: String) -> Self;
+    fn prop() -> Self;
+    fn ty() -> Self;
+}
+
+#[ext]
+impl<T: ConstructUsingNames> T {
+    fn forall_chain(
+        arguments: impl IntoIterator<Item = (Option<String>, Self)>,
+        return_type: Self,
+    ) -> Self {
+        let mut result = return_type;
+        for (name, ty) in arguments.collect::<Vec<_>>().into_iter().rev() {
+            result = Self::forall(name, ty, result)
+        }
+        result
+    }
+    fn lambda_chain(
+        arguments: impl IntoIterator<Item = (Option<String>, Self)>,
+        return_value: Self,
+    ) -> Self {
+        let mut result = return_value;
+        for (name, ty) in arguments.collect::<Vec<_>>().into_iter().rev() {
+            result = Self::lambda(name, ty, result)
+        }
+        result
+    }
+    fn apply_chain(f: Self, arguments: impl IntoIterator<Item = Self>) -> Self {
+        let mut result = f;
+        for argument in arguments {
+            result = Self::apply(result, argument)
+        }
+        result
+    }
+    fn variable(name: impl Into<String>) -> Self {
+        Self::variable_impl(name)
+    }
+}
+
+pub trait TermBuilder {
+    fn build(&self, context: &HashMap<String, Term>) -> Term;
+}
+
+pub struct Apply {
+    f: Box<dyn TermBuilder>,
+    args: Vec<Box<dyn TermBuilder>>,
+}
+
+pub struct Lambda {
+    args: Vec<(String, Box<dyn TermBuilder>)>,
+    body: Box<dyn TermBuilder>,
+}
+
+macro_rules! apply {
+    ($f:tt $args:tt+) => {
+        Apply{
+            f: Box::new($f),
+            args: vec![$(Box::new ($args))*]
+        }
+    }
+}
+
+macro_rules! lambda {
+    ($f:tt $body:tt+) => {
+        Lambda {
+            args: vec![$(Box::new ($args))*]
+        }
+    }
+}
+
+//pub fn lambda (name: impl ToString, body: )
+
+pub struct InductiveConstructor<T> {
+    name: String,
+    nonrecursive_arguments: Vec<(String, T)>,
+    // the data distinguishing each recursive argument is what the values of the indices are.
+    // this isn't fully general, but it's all I need for the construction of the Term and TypeJudgment types.
+    recursive_argument_indices: Vec<(String, Vec<T>)>,
+    return_indices: Vec<T>,
+}
+
+pub struct InductiveTypeDefinition<T> {
+    indices: Vec<(String, T)>,
+    constructors: Vec<InductiveConstructor<T>>,
+}
+
+pub struct InductiveTypeDefinitionGeneratedTerms<T> {
+    raw_type: T,
+    raw_constructors: Vec<(String, T)>,
+    induction_predicate: T,
+    induction_constructors: Vec<(String, T)>,
+    inductive_type: T,
+    inductive_constructors: Vec<(String, T)>,
+}
+
+impl<T: ConstructUsingNames + Clone> InductiveConstructor<T> {
+    pub fn raw_reducer_type(&self) -> T {
+        T::forall_chain(
+            self.nonrecursive_arguments
+                .iter()
+                .map(|(name, ty)| (None, ty.clone()))
+                .chain(
+                    self.recursive_argument_indices
+                        .iter()
+                        .map(|_| T::variable("P")),
+                ),
+            T::variable("P"),
+        )
+    }
+    pub fn inductive_reducer_type(&self, raw_type: &T) -> T {
+        T::forall_chain(
+            self.nonrecursive_arguments
+                .iter()
+                .map(|(name, ty)| (Some(name.clone()), ty.clone()))
+                .chain(
+                    self.recursive_argument_indices
+                        .iter()
+                        .flat_map(|index_values| {
+                            [
+                                T::apply_chain(raw_type.clone(), index_values.iter().cloned()),
+                                T::apply_chain(T::variable("P"), index_values.iter().cloned()),
+                            ]
+                        }),
+                ),
+            T::variable("P"),
+        )
+    }
+    pub fn raw_constructor_args(&self, raw_type: &T) -> impl Iterator<Item = (String, T)> {
+        constructor.nonrecursive_arguments.cloned().chain(
+            constructor
+                .recursive_argument_indices
+                .map(|(name, _ty)| (Some(name.clone()), raw_type.clone())),
+        )
+    }
+}
+
+impl<T: ConstructUsingNames + Clone> InductiveTypeDefinition<T> {
+    pub fn generate_terms(&self) -> InductiveTypeDefinitionGeneratedTerms<T> {
+        let raw_reducer_types: Vec<_> = self
+            .constructors
+            .iter()
+            .map(InductiveConstructor::raw_reducer_type)
+            .collect();
+        let raw_type = T::forall_chain(
+            iter::once((Some("P".into()), T::ty())).chain(raw_reducer_types.clone()),
+            T::variable("P"),
+        );
+
+        let raw_constructors: Vec<_> = self
+            .constructors
+            .iter()
+            .map(|constructor: &InductiveConstructor<T>| {
+                let args = constructor.raw_constructor_args(raw_type);
+                let value = T::lambda_chain(
+                    args.iter()
+                        .map(|(name, ty)| (Some(name.clone()), ty.clone()))
+                        .chain(
+                            iter::zip(&self.constructors, &raw_reducer_types)
+                                .map(|(c2, r2)| (Some(c2.name.clone()), r2)),
+                        ),
+                    T::apply_chain(
+                        T::variable(&constructor.name),
+                        args.into_iter().map(|name, _ty| T::variable(name)),
+                    ),
+                );
+                (format!("raw{}", constructor.name), value)
+            })
+            .collect();
+
+        let induction_predicate = T::forall_chain(
+            iter::once((Some("P".into()), T::ty())).chain(raw_reducer_types.clone()),
+            T::variable("P"),
+        );
+    }
+
+    pub fn term() -> Self {
+        InductiveTypeDefinition {
+            indices: vec![],
+            constructors: vec![
+                InductiveConstructor {
+                    name: "Prop".into(),
+                    nonrecursive_arguments: vec![],
+                    recursive_argument_indices: vec![],
+                    return_indices: vec![],
+                },
+                InductiveConstructor {
+                    name: "Type".into(),
+                    nonrecursive_arguments: vec![],
+                    recursive_argument_indices: vec![],
+                    return_indices: vec![],
+                },
+                InductiveConstructor {
+                    name: "Variable".into(),
+                    nonrecursive_arguments: vec![],
+                    recursive_argument_indices: vec![],
+                    return_indices: vec![],
+                },
+                InductiveConstructor {
+                    name: "ForAll".into(),
+                    nonrecursive_arguments: vec![],
+                    recursive_argument_indices: vec![
+                        ("ArgumentType".into(), vec![]),
+                        ("ReturnType".into(), vec![]),
+                    ],
+                    return_indices: vec![],
+                },
+                InductiveConstructor {
+                    name: "Lambda".into(),
+                    nonrecursive_arguments: vec![],
+                    recursive_argument_indices: vec![
+                        ("ArgumentType".into(), vec![]),
+                        ("ReturnValue".into(), vec![]),
+                    ],
+                    return_indices: vec![],
+                },
+                InductiveConstructor {
+                    name: "Apply".into(),
+                    nonrecursive_arguments: vec![],
+                    recursive_argument_indices: vec![
+                        ("Function".into(), vec![]),
+                        ("Argument".into(), vec![]),
+                    ],
+                    return_indices: vec![],
+                },
+            ],
+        }
+    }
+}
