coc-rs/src/lib.rs
@@ -1,6 +1,7 @@
 #![feature(default_free_fn, array_methods)]
 
 pub mod incomplete_term;
+pub mod inductive_type;
 pub mod term;
 pub mod types;
 
